\documentclass{article}

\begin{document}

\title{Math 130, 1.10 Problem 11}

\author{Martin Camacho}
\maketitle

Solve the following initial value problem:
\[ 
  y' = 4y - 1 \quad
  y(0) = 1  \quad h = 0.05 \quad \textrm{and} \quad y(0.5)
\]

Another first order linear ODE. This equation looks seperable:

\[y' = 4y - 1\]
\[\frac{dy}{dx} = 4y - 1\]
\[dy = (4y - 1)dx\]
\[\frac{1}{4y - 1}dy = dx\]

Now that we have all the \(y\)'s on the left and the \(x\)'s on the right, we can integrate:

\[ \int \frac{1}{4y - 1} \,dy = \int dx \]

Right side is trivial:

\[\int dx = x + C_1\]

The left side can be solved with substitution:

\[\textrm{Let} \quad u = 4y - 1 \quad du = 4dy \quad dy = \frac{du}{4}\]

Now do the substitution:

\[\int \frac{1}{4y - 1} \,dy = -\int \frac{1}{u} \,\frac{du}{4} = \frac{1}{4}\int \frac{1}{u} \,du = \frac{1}{4}(\ln(u) + C_2) = \frac{1}{4}(\ln(4y -1) + C_2)\]

Now putting both of the integrals together:

\[\frac{1}{4}(\ln(4y -1) = x + C_1\]
\[\ln(4y -1) + C_2 = 4x + 4C_1\]
\[\ln(4y -1) = 4x + C_3\]
\[4y - 1 = e^{4x + C_3}\]
\[4y = e^{4x + C_3} +1 \]

The general solution is:
\[y = \frac{1}{4}(e^{4x + C_3} +1 )\]

Using the initial value  \(y(0) = 1\), we can calculate  \(C_3\).

\[y(0) = 1 = \frac{1}{4}(e^{0 + C_3} +1 ) = \frac{1}{4}(e^{C_3} +1 )\]
\[4 = e^{C_3} + 1\]
\[3 = e^{C_3}\]
\[C_3 = \ln(3)\]

The particular solution is:
\[y = \frac{1}{4}(e^{4x + \ln(3)} +1 )\]

\end{document}